Tactics.v
@@ -1,0 +1,23 @@
+(** Destruct all hypotheses of the form [exists x, ...], while attempting
+    to preserve the name of the existensial variable. *)
+
+Ltac deex :=
+  repeat match goal with
+    | H: exists x, _ |- _ =>
+        let x' := fresh x in
+        destruct H as [x' H]
+  end.
+
+(** Destruct all disjunctive hypotheses. *)
+
+Ltac deor :=
+  repeat match goal with
+  | H: _ \/ _ |- _ => destruct H
+  end.
+
+(** Destruct all conjunctive hypotheses. *)
+
+Ltac deand :=
+  repeat match goal with
+  | H: _ /\ _ |- _ => destruct H
+  end.
