README.md
@@ -1,0 +1,13 @@
+# Proof of Church-Rosser in Martin-Löf's Type Theory
+
+This repository houses a small Coq proof that the [Church-Rosser][Church]
+theorem holds for Martin-Löf's intuitionistic theory of types.
+
+[church]: https://en.wikipedia.org/wiki/Church%E2%80%93Rosser_theorem
+
+## Building
+
+```
+$ coq_makefile -f _CoqProject -o Makefile
+$ make
+```
